% !TEX root = ../Tesis.tex
\chapter{Desarrollo del gradiente \texorpdfstring{$o_t$}{ot} y \texorpdfstring{$a_o$}{ao}}
\label{ApA}

Para $o_t$:

$\dfrac{E}{o_t} = \dfrac{\partial E}{\partial h_t} \cdot \dfrac{\partial h_t}{\partial o_t}$, por regla de la cadena

$\Longrightarrow \dfrac{E}{o_t} = \dfrac{\partial E}{\partial h_t} \cdot \dfrac{\partial}{\partial o_t} (o_t \cdot \tanh(c_t))$, sustituyendo el valor de $h_t$

$\Longrightarrow \dfrac{E}{o_t} = \dfrac{\partial E}{\partial h_t} \cdot \tanh(c_t)$

Y para $a_o$:

$\dfrac{E}{\partial a_o} = \dfrac{\partial E}{\partial o_t} \cdot \dfrac{\partial o_t}{\partial a_o}$

$\Longrightarrow \dfrac{E}{\partial a_o} = \dfrac{\partial E}{\partial o_t} \cdot \dfrac{\partial}{\partial a_o} (\sigma (a_o))$

$\Longrightarrow \dfrac{E}{\partial a_o} = \dfrac{\partial E}{\partial o_t} \cdot \sigma (a_o)(1-\sigma(a_o)$

$\Longrightarrow \dfrac{E}{\partial a_o} = \dfrac{\partial E}{\partial h_t} \cdot \tanh(c_t) \cdot o_t(1-o_t)$ 